work on pattern matching correctness
exp_to_Cexp_thm1 is almost ready now for application of as-yet-unproved
theorem relating Cevaluate_match and remove_mat_var. The latter's
statement probably needs to be changed to only reason up to syneq and to
state exactly which variables must be free for what or contained in
what before it can be proved.

examples/miniML/compiler/correctness/compileCorrectnessScript.sml
@@ -1164,11 +1164,6 @@ val (Cevaluate_match_rules,Cevaluate_match_ind,Cevaluate_match_cases) = Hol_reln
   (Cpnomatch p v ∧ Cevaluate_match v pes env r
     ⇒ Cevaluate_match v ((p,e)::pes) env r)`
 
-(*
-val Cevaluate_match_remove_mat_var = store_thm("Cevaluate_match_remove_mat_var",
-  ``
-*)
-
 val EVERY2_MAP = store_thm("EVERY2_MAP",
   ``(EVERY2 P (MAP f l1) l2 = EVERY2 (λx y. P (f x) y) l1 l2) ∧
     (EVERY2 Q l1 (MAP g l2) = EVERY2 (λx y. Q x (g y)) l1 l2)``,
@@ -1311,8 +1306,11 @@ val pmatch_Cpnomatch = store_thm("pmatch_Cpnomatch",
   strip_tac >- rw[pmatch_def] >>
   rw[pmatch_def])
 
+val matchres_def = Define`
+  matchres env cenv env' e r = ∃env''. (env' = env'' ++ env) ∧ (r = Rval (env'',e))`
+
 val evaluate_match_with_Cevaluate_match = store_thm("evaluate_match_with_Cevaluate_match",
-  ``∀pes r. evaluate_match_with (λcenv env' e r. ∃env''. (env' = env'' ++ env) ∧ (r = Rval (env'',e))) cenv env v pes r ⇒
+  ``∀pes r. evaluate_match_with (matchres env) cenv env v pes r ⇒
       ∀m. good_cenv cenv ∧ good_cmap cenv m ⇒
         ((r = Rerr (Rraise Bind_error))
             ⇒ Cevaluate_match (v_to_Cv m v)
@@ -1326,12 +1324,138 @@ val evaluate_match_with_Cevaluate_match = store_thm("evaluate_match_with_Cevalua
   strip_tac >- ( rw[] >> rw[Once Cevaluate_match_cases] ) >>
   strip_tac >- (
     rw[] >> rw[Once Cevaluate_match_cases] >>
+    fs[matchres_def] >>
     PROVE_TAC[pmatch_Cpmatch] ) >>
   strip_tac >- (
     rw[] >>
     rw[Once Cevaluate_match_cases] >>
     PROVE_TAC[pmatch_Cpnomatch] ) >>
   strip_tac >- rw[] >> rw[] )
+
+val evaluate_match_with_matchres = store_thm("evaluate_match_with_matchres",
+  ``∀pes r. evaluate_match_with P cenv env v pes r ⇒
+            (r ≠ Rerr Rtype_error) ⇒
+            ((r = Rerr (Rraise Bind_error)) ∧
+             evaluate_match_with (matchres env) cenv env v pes (Rerr (Rraise Bind_error))) ∨
+            ∃menv mr. evaluate_match_with (matchres env) cenv env v pes (Rval (menv,mr)) ∧
+                      P cenv (menv++env) mr r``,
+  ho_match_mp_tac evaluate_match_with_ind >>
+  strip_tac >- rw[Once evaluate_match_with_cases] >>
+  strip_tac >- (
+    rw[] >>
+    disj2_tac >>
+    rw[Once evaluate_match_with_cases] >>
+    rw[matchres_def] >>
+    fs[Once pmatch_nil] >>
+    Cases_on `pmatch cenv p v []` >>fs[] >>
+    PROVE_TAC[] ) >>
+  strip_tac >- (
+    rw[] >> fs[] >>
+    rw[Once evaluate_match_with_cases] >>
+    disj2_tac >>
+    rw[Once evaluate_match_with_cases] >>
+    PROVE_TAC[] ) >>
+  strip_tac >- rw[] >>
+  rw[])
+
+val evaluate_match_with_matchres_closed = store_thm("evaluate_match_with_matchres_closed",
+  ``∀pes r. evaluate_match_with (matchres env) cenv env v pes r ⇒
+            EVERY closed (MAP SND env) ∧ closed v ⇒
+            every_result (λ(menv,mr). EVERY closed (MAP SND menv) ∧
+                                      ∃p. MEM (p,mr) pes ∧
+                                          (set (MAP FST menv) = pat_vars p)) r ``,
+  ho_match_mp_tac evaluate_match_with_ind >>
+  strip_tac >- rw[] >>
+  strip_tac >- (
+    rw[matchres_def] >>
+    fs[] >>
+    fs[Once pmatch_nil] >>
+    Cases_on `pmatch cenv p v []` >> fs[] >>
+    qspecl_then [`cenv`,`p`,`v`,`[]`] mp_tac (CONJUNCT1 pmatch_closed) >>
+    fs[] >> fsrw_tac[DNF_ss][] ) >>
+  strip_tac >- (
+    rw[] >> fs[] >>
+    Cases_on `r` >> fs[] >>
+    fs[pairTheory.UNCURRY] >>
+    fsrw_tac[DNF_ss][] >> PROVE_TAC[]) >>
+  strip_tac >- rw[] >>
+  rw[])
+
+val Cevaluate_match_MAP_exp = store_thm("Cevaluate_match_MAP_exp",
+  ``∀pes env r. Cevaluate_match v pes env r ⇒
+      ∀f. Cevaluate_match v (MAP (λ(p,e). (p, f e)) pes) env (OPTION_MAP f r)``,
+  ho_match_mp_tac Cevaluate_match_ind >>
+  strip_tac >- rw[Once Cevaluate_match_rules] >>
+  strip_tac >- rw[Once Cevaluate_match_cases] >>
+  rw[] >>
+  rw[Once Cevaluate_match_cases])
+
+(*
+  probably need to reason up to syneq only, and
+  need to be clearer about which variable names are (contained in or fresh for)
+  where, so can more easily permute FUNIONs and FUPDATEs and stuff within the
+  proofs
+
+  val Cpmatch_remove_mat = store_thm("Cpmatch_remove_mat",
+    ``(∀p v menv. Cpmatch p v menv ⇒
+         ∀env x. (FLOOKUP env x = SOME v) ⇒
+           ∀fk e r. Cevaluate (menv ⊌ env) e r ⇒ Cevaluate env (remove_mat_vp fk e x p) r) ∧
+      (∀ps vs menv. Cpmatch_list ps vs menv ⇒
+         ∀env x c. (FLOOKUP env x = SOME (CConv c vs)) ⇒
+           ∀fk e n r. n ≤ LENGTH ps ∧ Cevaluate (menv ⊌ env) e r
+                        ⇒ Cevaluate env (remove_mat_con fk e x n (DROP n ps)) r)``,
+    ho_match_mp_tac Cpmatch_ind >>
+    strip_tac >- (
+      rw[remove_mat_var_def] >>
+      rw[Once Cevaluate_cases] >>
+      fs[FLOOKUP_DEF] >>
+      fs[FUNION_FUPDATE_1,FUNION_FEMPTY_1] ) >>
+    strip_tac >- (
+      rw[remove_mat_vp_def] >>
+      fs[FLOOKUP_DEF] >>
+      rw[Once Cevaluate_cases] >>
+      disj1_tac >>
+      qexists_tac `T` >>
+      fs[FUNION_FEMPTY_1] >>
+      rw[Once Cevaluate_cases] >>
+      rw[Cevaluate_list_with_Cevaluate,Cevaluate_list_with_cons] ) >>
+    strip_tac >- (
+      rw[] >>
+      rw[Once Cevaluate_cases] >>
+      disj1_tac >>
+      qexists_tac `T` >>
+      fs[] >>
+      conj_tac >- (
+        rw[Once Cevaluate_cases] >>
+        fs[FLOOKUP_DEF] ) >>
+      `ps = DROP 0 ps` by rw[] >>
+      pop_assum SUBST1_TAC >>
+      first_x_assum (match_mp_tac o MP_CANON) >>
+      rw[] >> PROVE_TAC[] ) >>
+    strip_tac >- rw[FUNION_FEMPTY_1] >>
+    rpt gen_tac >> strip_tac >>
+    rpt gen_tac >> strip_tac >>
+    ntac 2 gen_tac >>
+    Cases >- (
+      rw[] >>
+      rw[Once Cevaluate_cases] >>
+      disj1_tac >>
+      rw[Once Cevaluate_cases] >>
+      qpat_assum `FLOOKUP env x = Y` mp_tac >>
+      rw[FLOOKUP_DEF] >>
+
+  val Cevaluate_match_remove_mat_var = store_thm("Cevaluate_match_remove_mat_var",
+    ``∀pes menv mr. Cevaluate_match v pes menv mr ⇒
+        ∀env x. (FLOOKUP env x = SOME v) ⇒
+         case mr of
+         | NONE => Cevaluate env (remove_mat_var x pes) (Rerr (Rraise Bind_error))
+         | SOME e => ∀r. Cevaluate (menv ⊌ env) e r ⇒ Cevaluate env (remove_mat_var x pes) r``,
+    ho_match_mp_tac Cevaluate_match_ind >>
+    strip_tac >- rw[remove_mat_var_def] >>
+    strip_tac >- (
+      rw[remove_mat_var_def] >>
+      rw[Once Cevaluate_cases] >>
+*)
 
 val exp_to_Cexp_thm1 = store_thm("exp_to_Cexp_thm1",
   ``∀cenv env exp res. evaluate cenv env exp res ⇒
@@ -2017,42 +2141,68 @@ strip_tac >- (
   rpt strip_tac >> fs[] >>
   first_x_assum (qspec_then `m` mp_tac) >> rw[] >>
   qmatch_assum_rename_tac `syneq (v_to_Cv m v) w`[] >>
-  rw[exp_to_Cexp_def,LET_THM]
-
->> (*
-  gen_tac >>
-  CONV_TAC (RESORT_FORALL_CONV
-    (uncurry cons o pluck (equal "pes" o fst o dest_var))) >>
-  Induct >- (
-    rw[evaluate_match_with_evaluate] >>
-    rw[exp_to_Cexp_def,LET_THM] >>
-    rw[Once Cevaluate_cases] >>
-    rw[remove_mat_var_def] >>
-    fs[Once evaluate_match_with_cases] >>
-    rw[] >> PROVE_TAC[] ) >>
-  qx_gen_tac `pe` >>
-  fs[evaluate_match_with_evaluate] >>
   rw[exp_to_Cexp_def,LET_THM] >>
   rw[Once Cevaluate_cases] >>
-  fsrw_tac[DNF_ss][] >>
+  srw_tac[DNF_ss][] >>
   disj1_tac >>
-  first_x_assum (qspec_then `m` mp_tac) >>
-  rw[] >>
-  qmatch_assum_rename_tac `syneq (v_to_Cv m v) w`[] >>
   CONV_TAC SWAP_EXISTS_CONV >> qexists_tac `w` >> fs[] >>
-  fs[exp_to_Cexp_def,LET_THM] >>
-  qpat_assum `evaluate_match_with evaluate cenv env v p9 res` mp_tac >>
-  rw[Once evaluate_match_with_cases] >- (
-  
-    rw[pes_to_Cpes_MAP]
-    MiniMLTerminationTheory.pmatch_def
-  fs[evaluate_match_with_cases]
-
-  Induct_on `pes` >- (
-    fs[pes_to_Cpes_MAP,remove_mat_var_def] >>
-    fs[Once evaluate_match_with_cases] ) >>
-*) cheat) >>
-
+  qmatch_assum_abbrev_tac `evaluate_match_with P cenv env v pes res` >>
+  Q.ISPECL_THEN [`pes`,`res`] mp_tac evaluate_match_with_matchres >> fs[] >>
+  strip_tac >>
+  qmatch_assum_abbrev_tac `evaluate_match_with (matchres env) cenv env v pes r` >>
+  Q.ISPECL_THEN [`pes`,`r`] mp_tac evaluate_match_with_Cevaluate_match >>
+  fs[Abbr`r`] >>
+  disch_then (qspec_then `m` mp_tac) >>
+  rw[] >- (
+    qmatch_assum_abbrev_tac `Cevaluate_match vv ppes FEMPTY NONE` >>
+    `Cevaluate_match vv (MAP (λ(p,e). (p, exp_to_Cexp m e)) ppes) FEMPTY NONE` by (
+      metis_tac [Cevaluate_match_MAP_exp, optionTheory.OPTION_MAP_DEF] ) >>
+    qmatch_assum_abbrev_tac `Cevaluate_match vv (MAP ff ppes) FEMPTY NONE` >>
+    `MAP ff ppes = pes_to_Cpes m pes` by (
+      unabbrev_all_tac >>
+      rw[pes_to_Cpes_MAP,LET_THM] >>
+      rw[MAP_MAP_o,combinTheory.o_DEF,pairTheory.LAMBDA_PROD] >>
+      rw[pairTheory.UNCURRY] ) >>
+    fs[] >>
+    unabbrev_all_tac >>
+    pop_assum kall_tac >>
+    pop_assum mp_tac >>
+    pop_assum kall_tac >>
+    strip_tac >>
+    cheat (* Cevaluate_match_remove_mat_var *) ) >>
+  qmatch_assum_abbrev_tac `Cevaluate_match vv ppes eenv (SOME mr)` >>
+  `Cevaluate_match vv (MAP (λ(p,e). (p, exp_to_Cexp m e)) ppes) eenv (SOME (exp_to_Cexp m mr))` by (
+    metis_tac [Cevaluate_match_MAP_exp, optionTheory.OPTION_MAP_DEF] ) >>
+  pop_assum mp_tac >>
+  unabbrev_all_tac >>
+  pop_assum kall_tac >>
+  strip_tac >>
+  qmatch_assum_abbrev_tac `Cevaluate_match vv (MAP ff ppes) eenv mmr` >>
+  `MAP ff ppes = pes_to_Cpes m pes` by (
+    unabbrev_all_tac >>
+    rw[pes_to_Cpes_MAP,LET_THM] >>
+    rw[MAP_MAP_o,combinTheory.o_DEF,pairTheory.LAMBDA_PROD] >>
+    rw[pairTheory.UNCURRY] ) >>
+  fs[] >>
+  unabbrev_all_tac >>
+  pop_assum kall_tac >>
+  pop_assum mp_tac >>
+  pop_assum mp_tac >>
+  fs[] >>
+  `every_result closed (Rval v)` by (
+    match_mp_tac (MP_CANON evaluate_closed) >>
+    PROVE_TAC[] ) >>
+  Q.ISPECL_THEN [`pes`,`Rval (menv,mr)`] mp_tac evaluate_match_with_matchres_closed >>
+  fs[] >> strip_tac >>
+  `FV mr ⊆ set (MAP FST menv) ∪ set (MAP FST env)` by (
+    fsrw_tac[DNF_ss][SUBSET_DEF] >>
+    fsrw_tac[DNF_ss][pairTheory.FORALL_PROD,MEM_MAP,pairTheory.EXISTS_PROD] >>
+    fsrw_tac[DNF_ss][EXTENSION,MEM_MAP,pairTheory.EXISTS_PROD] >>
+    PROVE_TAC[] ) >>
+  fs[] >>
+  disch_then (qspec_then `m` mp_tac) >>
+  rw[] >>
+  cheat (* Cevaluate_match_remove_mat_var *) ) >>
 cheat)
 
 val Cpat_nice_ind =
